\documentclass{4320hw}
\usepackage{amsmath,amssymb,latexsym}
\usepackage{verbatim}
\newcommand{\exercise}[1]{\noindent {\bf Exercise #1.}}

\begin{document}

\name{James Russo and Shiven Srivastava}
\netid{jdr289 and ss2654}
\homework{1}

\maketitle

\begin{exercises}
\item
\begin{enumerate}
\item
See txt file

\item
See txt file

\item
See txt file

\item
See txt file

\item
$\rho(temp, (Sells \bowtie_{Sells.iid=Item.iid} Item) \bowtie_{storeid} (Sells \bowtie_{Sells.iid=Item.iid} Item) )$
\newline
$\rho(temp1, temp \bowtie_{storeid} temp)$
\newline
$\rho(tempf(2 \rightarrow iid1, 4 \rightarrow color1, 5 \rightarrow iid2, 7 \rightarrow color2, 8 \rightarrow iid3, 10 \rightarrow color3, 11 \rightarrow iid4, 13 \rightarrow color4),  temp1)$
\newline
$\rho(check1, \sigma_{color1 \neq color2 \neq color3 \neq color4} tempf)$
\newline
$\rho(check2, \sigma_{color1 \neq color2 \neq color3 } (\pi_{storeid,color1, color2,color3} tempf))$
\newline
$\rho(ans, \pi_{storeid} (check2) - \pi_{storeid} (check1) )$
\newline
Table ans is our final result

\item
Sells S1 and Sells S2
\newline
$\rho(temp1, \pi_{iid} (\sigma_{storeid=S2.storeid} Sells))$
\newline
$\rho(temp2, \pi_{storeid} (\sigma_{iid=temp1.storeid} Sells))$
\newline
$\rho(temp3, \pi_{S1.storeid, S2.storeid} (\sigma_{S1.storeid \neq temp2.storeid} (S1 \times S2)))$
\newline
$\rho(temp4(1 \rightarrow storeid1, 2 \rightarrow storeid2), temp3)$
\newline
$\rho(ans, \pi_{storeid1, storeid2} (\sigma_{storeid1>storeid2} temp4))$
\newline
Table ans is our final result

\item
$\rho(sells2, sells)$
\newline
$\rho(cross, sells2 \times sells)$
\newline
$\rho(cross2(1 \rightarrow iid1, 2 \rightarrow storeid1, 3 \rightarrow price1, 4 \rightarrow iid2, 5 \rightarrow storeid2, 6 \rightarrow price2), cross)$
\newline
$\rho(notmin1, \sigma_{price2>price1 \wedge iid2=iid1 \wedge storeid2 \neq storeid1} cross2 )$
\newline
$\rho(notmin2, \pi_{iid2, storeid2, price2} notmin1)$
\newline
$\rho(ans, Sells-notmin2)$
\newline
Table ans is our final result
\end{enumerate}

\item
see txt file

\item
\begin{enumerate}
\item
True
\newline
$\delta(\sigma_C (R))\equiv \sigma_C(\delta (R))$
\newline
LHS
\newline
$\delta(\sigma_C (R))\equiv \{t \in R \mid$ c is true for t  $\}$
\newline
$\sigma_C (R)\equiv \{kt \in R \mid$ k is the multiplicity of t and c is true for t $\}$
\newline
$R \equiv \{kt \in R \mid$ k is the multiplicity for t $\}$
\newline
RHS:
\newline
$\sigma_C(\delta (R)) \equiv \{ t \in R \mid$ where c is true for t $\}$
\newline
$\delta (R) \equiv \{ kt \in R \mid$ k is the multiplicity for t $\}$
\newline
$R \equiv \{ kt \in R \mid$ k is the multiplicity for t $\}$
\newline
$LHS \equiv RHS$

\item
True
\newline
$\delta (\pi_A (R)) \equiv \pi_A (\delta(R)) $
\newline
LHS:
\newline
$\delta (\pi_A (R)) \equiv \{ t[A] \mid t \in R \}$
\newline
$\pi_A (R) \equiv \{ kt[A] \mid kt \in R \mid $ k is the multiplicity of t $\}$
\newline
$R \equiv \{ kt \in R \mid $ k is the multiplicity of t$\}$
\newline
RHS:
\newline
$\pi_A (\delta(R)) \equiv \{ t[A] \mid t \in R\}$
\newline
$\\delta(R) \equiv \{  t \in R \}$
\newline
$R \equiv \{ kt \in R \mid $ k is the multiplicity of t$\}$
\newline
$LHS \equiv RHS$

\item
True
\newline
$\delta(R \times S) \equiv \delta(R) \times \delta(S)$
\newline
LHS:
\newline
$\delta(R \times S) \equiv \{ r \cdot s \mid r \in R \wedge s \in S\}$
\newline
$R \times S  \equiv \{k(r \cdot s) \mid r \in R \wedge s \in S \wedge $ k is the multiplicity of $(r \cdot s) \}$
\newline 
RHS:
\newline
$\delta(R) \times \delta(S) \equiv  \{ r \cdot s \mid r \in R \wedge s \in S\}$ 
\newline
$R \times \delta(S) \equiv \{ m(r) \cdot s \mid r \in R \wedge s \in S \wedge $ m is the multiplicity of r$\}$
\newline
$R \times S \equiv \{ m(r) \cdot n(s) \mid r \in R \wedge s \in S \wedge $ m is the multiplicity of r  and n is the multiplicity of s$\}$
\newline
$R \times S  \equiv \{k(r \cdot s) \mid r \in R \wedge s \in S \wedge $ k=mn is the multiplicity of $(r \cdot s) \}$
\newline
$LHS \equiv RHS$

\item
True
\newline
$\delta(R \bowtie_C S) \equiv \delta(R) \bowtie_C \delta(S)$
\newline
LHS:
\newline
$\delta(R \bowtie_C S) \equiv \delta( \sigma_C (R \times S))$
\newline
$\delta( \sigma_C (R \times S)) \equiv \{ r \cdot s \mid r \in R \wedge s \in S \wedge $ c is true for $r \cdot s\}$
\newline
$ \sigma_C (R \times S) \equiv \{ k(r \cdot s) \mid r \in R \wedge s \in S \wedge $ c is true for $r \cdot s \wedge $ k is the multiplictity of $ r\cdot s\}$
\newline
$R \times S  \equiv \{k(r \cdot s) \mid r \in R \wedge s \in S \wedge $ k=mn is the multiplicity of $(r \cdot s) \}$
\newline
RHS:
\newline
$\delta(R) \bowtie_C \delta(S) \equiv \{ r \cdot s \mid r \in R \wedge s \in S \wedge $ c is true for $r \cdot s\}$
\newline
$R  \bowtie_C \delta(S) \equiv \{ m(r) \cdot s \mid r \in R \wedge s \in S \wedge $ c is true for $m(r) \cdot s \wedge$ m is the multiplicity of r$\}$
\newline
$R  \bowtie_C S \equiv \{ m(r) \cdot n(s) \mid r \in R \wedge s \in S \wedge $ c is true for $m(r) \cdot s \wedge$ m is the multiplicity of r  and n is the multiplicity of s$\}$
\newline
$R  \bowtie_C S \equiv \{k(r \cdot s) \mid r \in R \wedge s \in S \wedge $c is true for $ k(r \cdot s) \wedge$ k=mn is the multiplicity of $(r \cdot s) \}$
\newline
$R  \bowtie_C S  \equiv \sigma_C (R \times S)$
\newline
$\sigma_C (R \times S) \equiv \{k(r \cdot s) \mid r \in R \wedge s \in S \wedge $c is true for $ k(r \cdot s) \wedge$ k=mn is the multiplicity of $(r \cdot s) \}$
\newline
$R \times S  \equiv \{k(r \cdot s) \mid r \in R \wedge s \in S \wedge $ k=mn is the multiplicity of $(r \cdot s) \}$
\newline
$LHS \equiv RHS$

\item
False
\newline
$\delta(R \cup_B S) \neq \delta(R) \cup_B \delta(S)$
\newline
$R=\{ (1,2), (1,2), (3,4)\}$ and $S=\{ (1,2), (3,4), (3,4) \}$
\newline
LHS:
\newline
$R \cup_B S= \{ 1,2), (1,2), (1,2), (3,4), (3,4), (3,4) \}$
\newline
$\delta(R \cup_B S) = \{ (1,2), (3,4) \}$
\newline
RHS:
\newline
$\delta(R)=\{ (1,2), (3,4) \}$ and $\delta(S)=\{ (1,2), (3,4) \}$
\newline
$\delta(R) \cup_B \delta(S)= \{(1,2),(1,2),(3,4),(3,4) \}$
\newline
$LHS \neq RHS$ so this is false

\item
True
\newline
LHS:
\newline
$\delta(R \cap_B S) \equiv \delta(R) \cap_B \delta(S)$
\newline
$\delta(R \cap_B S) \equiv \{ t \in R \vee t \in S \mid$ t occurs in both R and S$\}$
\newline
$R \cap_B S \equiv \{ kt \in R \vee t \in S \mid $t occurs in both R and S and k is the minimum number of occurrences of t in either R or S$\} $
\newline
RHS:
\newline
$\delta(R) \cap_B \delta(S) \equiv  \{ t \in R \vee t \in S \mid$ t occurs in both R and S$\}$
\newline
$R \cap_B \delta(S) \equiv \{ mt \in R \vee t \in S \mid $t occurs in both R and S and m is the amount of occurrense of t in R$\}$
\newline
$R \cap_B S \equiv \{ mt \in R \vee nt \in S \mid $ t occurs in both R and S and m is the amount of occurrense of t in R and n is the n amount of occurences of t in S$\}$
\newline
$R \cap_B S \equiv \{ kt \in R \vee t \in S \mid $t occurs in both R and S and k is the minimum number of occurrences of t in either R or S$\} $
\newline
$LHS \equiv RHS$

\item
False
\newline
$\delta(R-_B S ) \equiv \delta(R) -_B \delta(S)$
\newline
$R=\{ (1,2), (1,2), (3,4)\}$ and $S=\{ (1,2), (3,4), (3,4) \}$
\newline
LHS:
\newline
$R -_BS = \{ (1,2) \}$
\newline
$\delta(R -_B S)= \{ (1,2) \}$
\newline
RHS:
\newline
$\delta(R)=\{ (1,2), (3,4) \}$ and $\delta(S)=\{ (1,2), (3,4) \}$
\newline
$ \delta(R) -_B \delta(S)=\{ \}$ empty set
\newline
$LHS \neq RHS$

\end{enumerate}

\end{exercises}
\end{document}